finish equivalence proof between rec and itree

dimsum/itree/rec.v
@@ -58,7 +58,7 @@ Definition rec_expr_itree (e : expr) : itree (callE expr val +' moduleE rec_even
       set_rec_heap he';;
       Ret v
   | Call f es =>
-      vs ← ITree.flat_map (λ e, trigger (Recursion.Call e)) es;
+      vs ← ITree.flat_map call es;
       fns ← get_rec_fns;
       if fns !! f is Some fn then
         assume (length vs = length fn.(fd_args));;
@@ -96,74 +96,103 @@ Definition rec_itree : itree (moduleE rec_event rec_state) void :=
   ITree.bind (rec' rec_expr_itree (Waiting false)) (λ _, NB).
 
 Local Ltac go :=
-  clear_itree.
+  clear_itree; repeat itree_step.
 Local Ltac go_s :=
   tstep_s; go.
 Local Ltac go_i :=
   tstep_i; go.
 
-Lemma itree_tstep_bind_tau {E R} A h (x : itree _ A) cont:
-  ITreeTStep (E:=E) (R:=R) cont (ITree.bind (Tau x) h) (Tau (ITree.bind x h)).
-Proof. constructor. by rewrite unfold_bind. Qed.
-Global Hint Resolve itree_tstep_bind_tau : typeclass_instances.
+(** ** rec_itree_expr_inv
 
-Lemma itree_tstep_interp_ret {E} {R A B S} f x cont (h : S → _):
-  ITreeTStep (E:=E) (R:=R) cont (ITree.bind (interp (recursive' (A:=A) (B:=B) f) (Ret x)) h) (ITree.bind (Ret x) h).
-Proof. constructor. by rewrite interp_ret. Qed.
-Global Hint Resolve itree_tstep_interp_ret : typeclass_instances.
+    [rec_itree_expr_inv] is a version of [is_static_expr] for proving
+    the equivalence.
 
-Lemma itree_tstep_interp_bind {E} {R A B S} f g1 (g2 : B → _) cont (h : S → _):
-  ITreeTStep (E:=E) (R:=R) cont
-    (ITree.bind (interp (recursive' (A:=A) (B:=B) f) (ITree.bind g1 g2)) h)
-    (ITree.bind (interp (recursive' f) g1) (λ x,
-         ITree.bind (interp (recursive' f) (g2 x)) h)).
-Proof. constructor. by rewrite interp_bind bind_bind. Qed.
-Global Hint Resolve itree_tstep_interp_bind : typeclass_instances.
+    TODO: Define a version of is_static_expr that takes a predicate on
+    the head of the expression and lifts it to the whole expression. *)
+Local Fixpoint rec_itree_expr_inv (e : expr) : bool :=
+  match e with
+  | Var v => true
+  | Val v => true
+  | BinOp e1 o e2 => rec_itree_expr_inv e1 && rec_itree_expr_inv e2
+  | Load e1 => rec_itree_expr_inv e1
+  | Store e1 e2 => rec_itree_expr_inv e1 && rec_itree_expr_inv e2
+  | If e e1 e2 => rec_itree_expr_inv e && rec_itree_expr_inv e1 && rec_itree_expr_inv e2
+  | LetE v e1 e2 => rec_itree_expr_inv e1 && rec_itree_expr_inv e2
+  | Call f args => forallb rec_itree_expr_inv args
+  | AllocA _ e => rec_itree_expr_inv e
+  | FreeA _ e => false
+  | ReturnExt can_return_further e => false
+  | Waiting can_return => true
+  end.
 
-Lemma itree_tstep_interp_rec'_call {E} {R A B} f x (h : B → _):
-  ITreeTStep (E:=E) (R:=R) false
-    (ITree.bind (interp (recursive' (A:=A) (B:=B) f) (call x)) h)
-    (ITree.bind (Tau (rec' f x)) h).
+Local Lemma rec_itree_expr_inv_forallb vs:
+  forallb rec_itree_expr_inv (Val <$> vs).
+Proof. by apply forallb_True, Forall_fmap, Forall_true. Qed.
+
+Local Lemma rec_itree_expr_inv_subst x v e:
+  rec_itree_expr_inv e →
+  rec_itree_expr_inv (subst x v e).
 Proof.
-  constructor. rewrite interp_recursive'_call_eq.
-  do 3 f_equiv. setoid_rewrite tau_euttge. by rewrite bind_ret_r.
-Qed.
-Global Hint Resolve itree_tstep_interp_rec'_call : typeclass_instances.
-
-Class ITreeToTranslate {E1 E2 R} (i : itree E1 R) (H : E2 -< E1) (o : itree E2 R) := {
-    itree_to_translate : i ≅ translate (@resum _ _ _ _ H) o
-}.
-Global Hint Mode ITreeToTranslate + + + ! + - : typeclass_instances.
-
-Lemma itree_tstep_interp_rec'_inr {E} {R A B} f (g : itree (callE A B +' E) _)
-  (g' : itree E _) (h : B → _) cont :
-  ITreeToTranslate g _ g' →
-  ITreeTStep (E:=E) (R:=R) cont
-    (ITree.bind (interp (recursive' (A:=A) (B:=B) f) g) h)
-    (ITree.bind g' h).
-Proof.
-  move => [Heq]. constructor.
-  by rewrite Heq /= interp_translate /recursive' interp_trigger_h_ge.
-Qed.
-Global Hint Resolve itree_tstep_interp_rec'_inr : typeclass_instances.
-
-Global Instance ITreeToTranslate_assume_option E1 E2 R (o : option R) {HE1 : choiceE -< E1} (Hin : E1 -< E2) {HE2 : choiceE -< E2} :
-  (∀ T, TCEq (HE2 T) (cat (@resum _ _ _ _ HE1) (@resum _ _ _ _ Hin) T)) →
-  ITreeToTranslate (assume_option o) Hin (assume_option o).
-Proof.
-  move => /(_ void)/TCEq_eq Heq.
-  constructor. destruct o => //=.
-  - by rewrite translate_ret.
-  - rewrite /UB translate_bind /angelic translate_trigger_eq.
-    f_equiv; [|done]. by rewrite /subevent/resum/= Heq.
+  elim: e => //= *; try naive_solver.
+  - by case_bool_decide.
+  - case_bool_decide; naive_solver.
+  - apply forallb_True, Forall_forall => ? /elem_of_list_fmap[?[??]]. subst.
+    revert select (Forall _ _) => /Forall_forall.
+    revert select (Is_true (forallb _ _)) => /forallb_True/Forall_forall. naive_solver.
 Qed.
 
+Local Lemma rec_itree_expr_inv_subst_l xs vs e:
+  rec_itree_expr_inv e →
+  rec_itree_expr_inv (subst_l xs vs e).
+Proof.
+  elim: xs vs e. { by case. }
+  move => ?? IH [//|??] /=??. apply IH.
+  by apply rec_itree_expr_inv_subst.
+Qed.
 
-Lemma itree_tstep_rec' {E} {R A B} f x  (h : B → _):
-  ITreeTStep (E:=E) (R:=R) false (ITree.bind (rec' (A:=A) (B:=B) f x) h) (ITree.bind (interp (recursive' f) (f x)) h).
-Proof. constructor. by rewrite rec'_as_interp_eq. Qed.
-Global Hint Resolve itree_tstep_rec' : typeclass_instances.
+Local Lemma is_static_expr_rec_itree_expr_inv e:
+  is_static_expr false e →
+  rec_itree_expr_inv e.
+Proof.
+  elim: e => //=; try naive_solver.
+  move => ?? IH /forallb_True.
+  elim: IH => // *. decompose_Forall_hyps; naive_solver.
+Qed.
 
+(** ** equivalence proof *)
+Lemma rec_itree_refines_rec_call t e h fns k K f args b n:
+  t ⊒ ↓ᵢ (ITree.bind (interp (recursive' rec_expr_itree) (ITree.flat_map call args)) k) →
+  (∀ t' e' h' K' a k,
+      a ∈ args →
+      t' ⊒ ↓ᵢ (Tau (ITree.bind (rec' rec_expr_itree a) k)) →
+      (∀ t'' e'' h'' v,
+          t'' ⊒ ↓ᵢ (k v) →
+          (t'', Rec e'' h'' fns) ⪯{itree_trans rec_event rec_state, rec_trans, n, b}
+            Rec (expr_fill K' (Val v)) h'' fns) →
+      (t', Rec e' h' fns) ⪯{itree_trans rec_event rec_state, rec_trans, n, b}
+        Rec (expr_fill K' a) h' fns) →
+  (∀ t' e' h' argsv,
+      t' ⊒ ↓ᵢ (k argsv) →
+      (t', Rec e' h' fns) ⪯{itree_trans rec_event rec_state, rec_trans, n, b}
+        Rec (expr_fill K (Call f (Val <$> argsv))) h' fns) →
+  (t, Rec e h fns) ⪯{itree_trans rec_event rec_state, rec_trans, n, b}
+    Rec (expr_fill K (Call f args)) h fns.
+Proof.
+  move => Ht Hargs Hret. move: Ht Hargs.
+  change args with ((Val <$> []) ++ args) at 3.
+  change k with (λ x, k ([] ++ x)).
+  move: (@nil val) => argsv.
+  elim: args argsv h e t.
+  { move => argsv h e t /= Ht ?. go. move: Ht. rewrite !app_nil_r. naive_solver. }
+  move => /= arg args IH argsv h e t Ht Ha.
+  go_i. change (Call _ _) with (expr_fill ([CallCtx f argsv args]) arg).
+  rewrite -expr_fill_app. eapply Ha; [set_solver|done|].
+  move => ??? /=??. rewrite cons_middle app_assoc -fmap_snoc.
+  apply IH; [|set_solver].
+  etrans; [done|].
+  rewrite interp_bind bind_bind. setoid_rewrite interp_ret.
+  setoid_rewrite bind_ret_l. do 2 f_equiv. move => ?. by rewrite <-app_assoc.
+Qed.
 
 Lemma rec_itree_refines_rec fns :
   trefines (itree_mod rec_itree (rec_init fns)) (rec_mod fns).
@@ -174,26 +203,226 @@ Proof.
     ∃ K e k,
     t ⊒ ↓ᵢ (ITree.bind (rec' rec_expr_itree e) k) ∧
     RecExprFill es K e ∧ hi = hs ∧ fnsi = fns ∧ fnss = fns ∧
-    ∀ v t' ei h', t' ⊒ ↓ᵢ (k v) → (t', Rec ei h' fns) ⪯{itree_trans rec_event rec_state, rec_trans, n, false} Rec (expr_fill K (Val v)) h' fns). }
-  { exists []. split!; [done|apply _|]. move => ?????/=. by go_i. } {
+    rec_itree_expr_inv e ∧
+    ∀ v t' ei h' b, t' ⊒ ↓ᵢ (k v) → (t', Rec ei h' fns) ⪯{itree_trans rec_event rec_state, rec_trans, n, b} Rec (expr_fill K (Val v)) h' fns). }
+  { exists []. split!; [done|apply _|done|]. move => ??????/=. by go_i. } {
     move => ?? [?[???]] [???] ? /= ?. destruct!. split!; [done..|]. move => *. apply: tsim_mono; naive_solver. }
-  move => n /= ? Hloop [?[???]] [???] [? [e ?]]. destruct!/=. go_i.
+  move => n /= ? Hloop [?[???]] [???] [? [e ?]]. destruct!/=.
+  rename H6 into Hret. go_i.
   revert select (RecExprFill _ _ _) => -[?].
   destruct e; simplify_eq/=.
   - by tstep_s.
-  - go_i. by apply H5.
+  - go_i. by apply Hret.
   - go_i. go_i.
-    apply Hloop; [done|]. split!; [done|apply _|].
-    move => /= *.
+    apply Hloop; [done|]. split!; [done|apply _|naive_solver|].
+    move => /= *. go.
     go_i. go_i.
-    apply Hloop; [done|]. split!; [done|apply _|].
-    move => /= *.
+    apply Hloop; [done|]. split!; [done|apply _|naive_solver|].
+    move => /= *. go.
     go_s => ??.
     go_i. split!. go.
-    go_i. by apply H5.
+    by apply Hret.
   - go_i. go_i.
-    apply Hloop; [done|]. split!; [done|apply _|].
-    move => /= *.
+    apply Hloop; [done|]. split!; [done|apply _|naive_solver|].
+    move => /= *. go.
     go_s => *. simplify_eq/=.
-    go_i.
-Abort.
+    go_i. go_i. split!. go.
+    by apply Hret.
+  - go. go_i. go_i.
+    apply Hloop; [done|]. split!; [done|apply _|naive_solver|].
+    move => /= *. go.
+    go_i. go_i.
+    apply Hloop; [done|]. split!; [done|apply _|naive_solver|].
+    move => /= *. go.
+    go_s => *. simplify_eq/=. go.
+    go_i. go_i. split!. go. go_i. go_i.
+    by apply Hret.
+  - go. go_i. go_i.
+    apply Hloop; [done|]. split!; [done|apply _|naive_solver|].
+    move => /= *. go.
+    go_s => b *. simplify_eq/=. go_i.
+    destruct b; go_i; go_i.
+    all: apply Hloop; [done|]; split!; [done|apply _|naive_solver|done].
+  - go. go_i. go_i.
+    apply Hloop; [done|]. split!; [done|apply _|naive_solver|].
+    move => /= *. go.
+    go_s.
+    go_i. go_i.
+    apply Hloop; [done|].
+    split!; [done|apply _|apply rec_itree_expr_inv_subst; naive_solver|done].
+  - go. revert select (Is_true (forallb _ _)) => /forallb_True/Forall_forall?.
+    apply: rec_itree_refines_rec_call; [done|..]. {
+      move => ???????? Hret2. go_i. apply Hloop; [done|].
+      split!; [done|apply _|naive_solver| ].
+      move => /= *. apply tsim_mono_b_false. naive_solver.
+    }
+    move => /= ?????. go_i.
+    case_match.
+    + go_s. split!. move => ?. go_i. split!. go. go_i. go_i.
+      apply Hloop; [done|].
+      split!; [done|apply _| |done].
+      cbn. apply rec_itree_expr_inv_subst_l.
+      apply is_static_expr_rec_itree_expr_inv. apply fd_static.
+    + go_i. go_i. go_s. split!. go_i. go_i.
+      apply Hloop; [done|]. split!; [done|apply _|done|done].
+  - go.
+    destruct (decide (Forall (λ x : Z, 0 < x) ls.*2)).
+    2: { go_s. exploit (heap_alloc_list_fresh ls.*2 ∅) => -[??]. by split!. }
+    go_i. split!. go. go_i.
+    go_i => ?. go.
+    go_i => ?. go.
+    go_i => ?. go.
+    go_i. go_i. go_i. go_i.
+    go_s. split!; [done|]. move => ?.
+    apply Hloop; [done|]. split!; [done|apply _| |].
+    { move => *. apply rec_itree_expr_inv_subst_l. naive_solver. }
+    move => /= *. go.
+    go_s => ??.
+    go_i. go_i. split!. go. go_i. split!; [done|]. go.
+    go_i. go_i.
+    by apply Hret.
+  - done.
+  - done.
+  - go_i => b. go.
+    destruct b.
+    + go_i. go_i => ?. go. go_i => ?. go. go_i => ?. go.
+      go_i => ??. go. go_i. go_i. go_i.
+      go_s. split!. go_i. go_i.
+      apply Hloop; [done|]. split!; [done|apply _| |].
+      { move => /=. apply rec_itree_expr_inv_forallb. }
+      move => /= *. go.
+      go_i. go_i.
+      go_s. split!.
+      go_i. go_i.
+      apply Hloop; [done|]. split!; [done|apply _|done|done].
+    + go_i => ?. go. simplify_eq. go_i => ?. go. go_i => ?. go. go_i. go_i.
+      go_i. go_s. split!.
+      by apply Hret.
+Qed.
+
+Lemma rec_refines_rec_itree_call t e h fns k K f args b n:
+  t ⊒ ↓ᵢ (ITree.bind (interp (recursive' rec_expr_itree) (ITree.flat_map call args)) k) →
+  (∀ t' e' h' K' a k,
+      a ∈ args →
+      t' ⊒ ↓ᵢ (Tau (ITree.bind (rec' rec_expr_itree a) k)) →
+      (∀ t'' e'' h'' v,
+          t'' ⊒ ↓ᵢ (k v) →
+           (Rec (expr_fill K' (Val v)) h'' fns) ⪯{rec_trans, itree_trans rec_event rec_state, n, b}
+            (t'', Rec e'' h'' fns)) →
+       Rec (expr_fill K' a) h' fns ⪯{rec_trans, itree_trans rec_event rec_state, n, b}
+        (t', Rec e' h' fns)) →
+  (∀ t' e' h' argsv,
+      t' ⊒ ↓ᵢ (k argsv) →
+      (Rec (expr_fill K (Call f (Val <$> argsv))) h' fns)
+        ⪯{rec_trans, itree_trans rec_event rec_state, n, b}
+        (t', Rec e' h' fns)) →
+  (Rec (expr_fill K (Call f args)) h fns) ⪯{rec_trans, itree_trans rec_event rec_state, n, b}
+    (t, Rec e h fns).
+Proof.
+  move => Ht Hargs Hret. move: Ht Hargs.
+  change args with ((Val <$> []) ++ args) at 3.
+  change k with (λ x, k ([] ++ x)).
+  move: (@nil val) => argsv.
+  elim: args argsv h e t.
+  { move => argsv h e t /= Ht ?. go. move: Ht. rewrite !app_nil_r. naive_solver. }
+  move => /= arg args IH argsv h e t Ht Ha.
+  go_s. change (Call _ _) with (expr_fill ([CallCtx f argsv args]) arg).
+  rewrite -expr_fill_app. eapply Ha; [set_solver|done|].
+  move => ??? /=??. rewrite cons_middle app_assoc -fmap_snoc.
+  apply IH; [|set_solver].
+  etrans; [done|].
+  rewrite interp_bind bind_bind. setoid_rewrite interp_ret.
+  setoid_rewrite bind_ret_l. do 2 f_equiv. move => ?. by rewrite <-app_assoc.
+Qed.
+
+Lemma rec_refines_rec_itree fns :
+  trefines (rec_mod fns) (itree_mod rec_itree (rec_init fns)).
+Proof.
+  apply: tsim_implies_trefines => n0 /=.
+  rewrite /rec_itree.
+  unshelve eapply tsim_remember. { simpl. exact (λ n '(Rec ei hi fnsi) '(t, Rec _ hs fnss),
+    ∃ K e k,
+    t ⊒ ↓ᵢ (ITree.bind (rec' rec_expr_itree e) k) ∧
+    RecExprFill ei K e ∧ hi = hs ∧ fnsi = fns ∧ fnss = fns ∧
+    rec_itree_expr_inv e ∧
+    ∀ v t' ei h' b, t' ⊒ ↓ᵢ (k v) → Rec (expr_fill K (Val v)) h' fns ⪯{rec_trans, itree_trans rec_event rec_state, n, b} (t', Rec ei h' fns)). }
+  { exists []. split!; [done|apply _|done|]. move => ??????/=. by go_i. } {
+    move => ?? [???] [?[???]] ? /= ?. destruct!. split!; [done..|]. move => *. apply: tsim_mono; naive_solver. }
+  move => n /= ? Hloop [ei hi fnsi] [t [es hs fnss]] [K [e]].
+  elim/rec_expr_depth_ind: e ei hi fnsi t es hs fnss K.
+  move => e IHe *. destruct!/=.
+  rename H6 into Hret. revert select (RecExprFill _ _ _) => -[?]. subst.
+  destruct e; simplify_eq/=.
+  - go_s. by go_s.
+  - go_s. by apply Hret.
+  - go_s. go_s. go_s.
+    eapply IHe; [|split!; [done|apply _|naive_solver|]]; [lia|].
+    move => /= *. go_s. go_s.
+    apply tsim_mono_b_false.
+    eapply IHe; [|split!; [done|apply _|naive_solver|]]; [lia|].
+    move => /= *. go_s => ??. go.
+    go_i. split!. by apply Hret.
+  - go_s. go_s. go_s.
+    eapply IHe; [|split!; [done|apply _|naive_solver|]]; [lia|].
+    move => /= v *. go_s => ??. go. go_s. go_s => ??. go.
+    destruct v => //; simplify_eq/=.
+    go_i. split!. by apply Hret.
+  - go_s. go_s. go_s.
+    eapply IHe; [|split!; [done|apply _|naive_solver|]]; [lia|].
+    move => /= v *. go_s. go_s.
+    apply tsim_mono_b_false.
+    eapply IHe; [|split!; [done|apply _|naive_solver|]]; [lia|].
+    move => /= *. go_s => ??. go. go_s. go_s => ?. go. go_s. go_s.
+    destruct v => //; simplify_eq/=.
+    go_i. split!. by apply Hret.
+  - go_s. go_s. go_s.
+    eapply IHe; [|split!; [done|apply _|naive_solver|]]; [lia|].
+    move => /= v *. go_s => b ?. go.
+    destruct v; simplify_eq/=. destruct b; go_s; go_s.
+    + go_i. apply tsim_mono_b_false.
+      eapply IHe; [|split!; [done|apply _|naive_solver|]]; [lia|done].
+    + go_i. apply tsim_mono_b_false.
+      eapply IHe; [|split!; [done|apply _|naive_solver|]]; [lia|done].
+  - go_s. go_s. go_s.
+    eapply IHe; [|split!; [done|apply _|naive_solver|]]; [lia|].
+    move => /= *. go_s. go_s. go_i.
+    apply tsim_mono_b_false.
+    eapply IHe; [|split!; [done|apply _| |done]].
+    + rewrite rec_expr_depth_subst. lia.
+    + apply rec_itree_expr_inv_subst. naive_solver.
+  - revert select (Is_true (forallb _ _)) => /forallb_True/Forall_forall?.
+    go_s. apply: rec_refines_rec_itree_call; [done|..]. {
+      move => ???? a ??? Hret2. go_s.
+      eapply IHe; [|split!; [done|apply _|naive_solver|]].
+      { exploit (max_list_elem_of_le (rec_expr_depth a) (rec_expr_depth <$> args)); [|lia].
+        apply elem_of_list_fmap. naive_solver. }
+      move => /= *. apply tsim_mono_b_false. naive_solver.
+    }
+    move => /= *. go_s. tstep_both. split => *; simplify_option_eq.
+    + go_s => ?. go. tend. split!. go_s. go_s.
+      apply Hloop; [done|]. split!; [done|apply _| |done].
+      cbn. apply rec_itree_expr_inv_subst_l.
+      apply is_static_expr_rec_itree_expr_inv. apply fd_static.
+    + go_s. go_s. split!; [done|]. go. tend. go_s. go_s.
+      apply Hloop; [done|]. split!; [done|apply _|done|done].
+  - go_s. go_s => ?. go. go_i => *. split!.
+    go_s. go_s. eexists _. go. go_s. eexists _. go. go_s. split!; [done|]. go.
+    go_s. go_s. go_s. go_s.
+    apply Hloop; [done|]. split!; [done|apply _|apply rec_itree_expr_inv_subst_l; naive_solver |].
+    move => /= *. go_s. go_s => ?. go. go_s => ?. go. go_s. go_s.
+    go_i. split!; [done|].
+    by apply Hret.
+  - done.
+  - done.
+  - go_i. split.
+    + move => *. go_s. go_s. eexists true. go. go_s. go_s. eexists _. go.
+      go_s. eexists _. go. go_s. eexists _. go. go_s. split!; [done|]. go.
+      go_s. go_s. go_s. split!. go. go_s. go_s.
+      apply Hloop; [done|]. split!; [done|apply _|apply rec_itree_expr_inv_forallb|].
+      move => /= *. go_s.
+      go_i. go_s. split!. go. go_s. go_s.
+      apply Hloop; [done|]. split!; [done|apply _|done|done].
+    + move => ???. go_s. go_s. eexists false. go. go_s. split!; [by destruct can_return|]. go.
+      go_s. eexists _. go. go_s. eexists _. go. go_s. go_s. go_s. split!. go.
+      by apply Hret.
+Qed.
