dimsum/itree/events.v
@@ -19,6 +19,24 @@ Definition set_state {E S} `{!stateE S -< E} (s : S) : itree E unit :=
 Definition yield {E S} `{!stateE S -< E} : itree E unit :=
   (trigger EYield)%itree.
 
+Global Instance ITreeToTranslate_get_state E1 E2 S
+  {HE1 : stateE S -< E1} (Hin : E1 -< E2) {HE2 : stateE S -< E2} :
+  TCEq (HE2 S) (cat (@resum _ _ _ _ HE1) (@resum _ _ _ _ Hin) S) →
+  ITreeToTranslate (get_state) Hin (get_state).
+Proof. intros Heq%TCEq_eq. apply ITreeToTranslate_trigger. by rewrite Heq. Qed.
+
+Global Instance ITreeToTranslate_set_state E1 E2 S x
+  {HE1 : stateE S -< E1} (Hin : E1 -< E2) {HE2 : stateE S -< E2} :
+  TCEq (HE2 unit) (cat (@resum _ _ _ _ HE1) (@resum _ _ _ _ Hin) unit) →
+  ITreeToTranslate (set_state x) Hin (set_state x).
+Proof. intros Heq%TCEq_eq. apply ITreeToTranslate_trigger. by rewrite Heq. Qed.
+
+Global Instance ITreeToTranslate_yield E1 E2 S
+  {HE1 : stateE S -< E1} (Hin : E1 -< E2) {HE2 : stateE S -< E2} :
+  (TCEq (HE2 unit) (cat (@resum _ _ _ _ HE1) (@resum _ _ _ _ Hin) unit)) →
+  ITreeToTranslate yield Hin yield.
+Proof. intros Heq%TCEq_eq. apply ITreeToTranslate_trigger. by rewrite Heq. Qed.
+
 Global Typeclasses Opaque get_state set_state yield.
 
 (** * choice events *)
@@ -55,7 +73,62 @@ x1 → P x2 → x1 = x2]. *)
 Definition demonic_non_empty {E R} `{!choiceE -< E} (P : R → Prop) : itree E R :=
   (assume (∃ x, P x);; x ← demonic _; assert (P x);; Ret x)%itree.
 
-Global Typeclasses Opaque angelic demonic assume assert UB NB assume_option assert_option.
+
+Global Instance ITreeToTranslate_angelic E1 E2 T
+  {HE1 : choiceE -< E1} (Hin : E1 -< E2) {HE2 : choiceE -< E2} :
+  TCEq (HE2 T) (cat (@resum _ _ _ _ HE1) (@resum _ _ _ _ Hin) T) →
+  ITreeToTranslate (angelic T) Hin (angelic T).
+Proof. intros Heq%TCEq_eq. apply ITreeToTranslate_trigger. by rewrite Heq. Qed.
+
+Global Instance ITreeToTranslate_demonic E1 E2 T
+  {HE1 : choiceE -< E1} (Hin : E1 -< E2) {HE2 : choiceE -< E2} :
+  TCEq (HE2 T) (cat (@resum _ _ _ _ HE1) (@resum _ _ _ _ Hin) T) →
+  ITreeToTranslate (demonic T) Hin (demonic T).
+Proof. intros Heq%TCEq_eq. apply ITreeToTranslate_trigger. by rewrite Heq. Qed.
+
+Global Instance ITreeToTranslate_assume E1 E2 (P : Prop)
+  {HE1 : choiceE -< E1} (Hin : E1 -< E2) {HE2 : choiceE -< E2} :
+  TCEq (HE2 P) (cat (@resum _ _ _ _ HE1) (@resum _ _ _ _ Hin) P) →
+  ITreeToTranslate (assume P) Hin (assume P).
+Proof. intros Heq. unfold assume. apply _. Qed.
+
+Global Instance ITreeToTranslate_assert E1 E2 (P : Prop)
+  {HE1 : choiceE -< E1} (Hin : E1 -< E2) {HE2 : choiceE -< E2} :
+  TCEq (HE2 P) (cat (@resum _ _ _ _ HE1) (@resum _ _ _ _ Hin) P) →
+  ITreeToTranslate (assert P) Hin (assert P).
+Proof. intros Heq. unfold assert. apply _. Qed.
+
+Global Instance ITreeToTranslate_UB E1 E2 R
+  {HE1 : choiceE -< E1} (Hin : E1 -< E2) {HE2 : choiceE -< E2} :
+  TCEq (HE2 void) (cat (@resum _ _ _ _ HE1) (@resum _ _ _ _ Hin) void) →
+  ITreeToTranslate (R:=R) UB Hin UB.
+Proof. intros Heq. unfold UB. apply ITreeToTranslate_bind; [apply _|done]. Qed.
+
+Global Instance ITreeToTranslate_NB E1 E2 R
+  {HE1 : choiceE -< E1} (Hin : E1 -< E2) {HE2 : choiceE -< E2} :
+  TCEq (HE2 void) (cat (@resum _ _ _ _ HE1) (@resum _ _ _ _ Hin) void) →
+  ITreeToTranslate (R:=R) NB Hin NB.
+Proof. intros Heq. unfold NB. apply ITreeToTranslate_bind; [apply _|done]. Qed.
+
+Global Instance ITreeToTranslate_assume_option E1 E2 R (o : option R)
+  {HE1 : choiceE -< E1} (Hin : E1 -< E2) {HE2 : choiceE -< E2} :
+  TCEq (HE2 void) (cat (@resum _ _ _ _ HE1) (@resum _ _ _ _ Hin) void) →
+  ITreeToTranslate (assume_option o) Hin (assume_option o).
+Proof. intros ?. destruct o; simpl; apply _. Qed.
+
+Global Instance ITreeToTranslate_assert_option E1 E2 R (o : option R)
+  {HE1 : choiceE -< E1} (Hin : E1 -< E2) {HE2 : choiceE -< E2} :
+  TCEq (HE2 void) (cat (@resum _ _ _ _ HE1) (@resum _ _ _ _ Hin) void) →
+  ITreeToTranslate (assert_option o) Hin (assert_option o).
+Proof. intros ?. destruct o; simpl; apply _. Qed.
+
+Global Instance ITreeToTranslate_demonic_non_empty E1 E2 R (P : R → _)
+  {HE1 : choiceE -< E1} (Hin : E1 -< E2) {HE2 : choiceE -< E2} :
+  (∀ T, TCEq (HE2 T) (cat (@resum _ _ _ _ HE1) (@resum _ _ _ _ Hin) T)) →
+  ITreeToTranslate (demonic_non_empty P) Hin (demonic_non_empty P).
+Proof. intros ?. apply _. Qed.
+
+Global Typeclasses Opaque angelic demonic assume assert UB NB assume_option assert_option demonic_non_empty.
 
 (** * visible events *)
 Inductive visibleE (EV : TypeState) : TypeBelowState → TypeState :=
@@ -64,6 +137,12 @@ Arguments EVisible {_} _.
 
 Definition visible {E EV} `{!visibleE EV  -< E} (e : EV) : itree E unit :=
   (trigger (EVisible e))%itree.
+
+Global Instance ITreeToTranslate_visible EV E1 E2 e
+  {HE1 : visibleE EV -< E1} (Hin : E1 -< E2) {HE2 : visibleE EV -< E2} :
+  TCEq (HE2 unit) (cat (@resum _ _ _ _ HE1) (@resum _ _ _ _ Hin) unit) →
+  ITreeToTranslate (visible e) Hin (visible e).
+Proof. intros Heq%TCEq_eq. apply ITreeToTranslate_trigger. by rewrite Heq. Qed.
 
 Global Typeclasses Opaque visible.
 
